Provide standalone binaries
Fixes #1724

Note that we keep the non-unified binaries (and use them to build
generated files) to avoid OOMs on Coq's CI.

It's unfortunate that compilation is so slow here, taking almost an hour
on my machine just to extract and compile the various binaries.

<details><summary>Timing Diff</summary>
<p>

```
     Time |   Peak Mem | File Name
----------------------------------------------------------------------------------
53m02.47s | 2463008 ko | Total Time / Peak Mem
----------------------------------------------------------------------------------
 2m21.70s | 2462928 ko | ExtractionOCaml/fiat_crypto
 2m19.85s | 2463008 ko | ExtractionOCaml/bedrock2_fiat_crypto
 1m53.82s | 1863716 ko | ExtractionOCaml/solinas_reduction
 1m36.75s | 2462904 ko | ExtractionOCaml/with_bedrock2_fiat_crypto
 1m33.30s | 2316820 ko | ExtractionOCaml/bedrock2_fiat_crypto.ml
 1m30.98s | 2300660 ko | ExtractionOCaml/fiat_crypto.ml
 1m30.25s | 2075840 ko | ExtractionOCaml/with_bedrock2_word_by_word_montgomery
 1m26.51s | 2074640 ko | ExtractionOCaml/bedrock2_word_by_word_montgomery
 1m25.26s | 1829432 ko | ExtractionOCaml/word_by_word_montgomery
 1m22.38s | 1780504 ko | ExtractionOCaml/bedrock2_unsaturated_solinas
 1m20.72s | 2147524 ko | ExtractionOCaml/bedrock2_solinas_reduction
 1m20.62s | 2336764 ko | ExtractionOCaml/with_bedrock2_fiat_crypto.ml
 1m18.57s | 1416332 ko | ExtractionOCaml/with_bedrock2_base_conversion
 1m16.74s | 1469000 ko | ExtractionOCaml/bedrock2_dettman_multiplication
 1m14.80s | 1780196 ko | ExtractionOCaml/with_bedrock2_unsaturated_solinas
 1m14.67s | 1415232 ko | ExtractionOCaml/base_conversion
 1m08.91s | 1416276 ko | ExtractionOCaml/bedrock2_base_conversion
 1m08.90s | 1415436 ko | ExtractionOCaml/dettman_multiplication
 1m07.90s | 1415368 ko | ExtractionOCaml/saturated_solinas
 1m07.63s | 1525784 ko | ExtractionOCaml/unsaturated_solinas
 1m07.23s | 1449720 ko | ExtractionOCaml/with_bedrock2_dettman_multiplication
 1m07.09s | 1447196 ko | ExtractionOCaml/with_bedrock2_saturated_solinas
 1m07.02s | 1439752 ko | ExtractionOCaml/bedrock2_saturated_solinas
 1m06.29s | 1448860 ko | ExtractionOCaml/with_bedrock2_solinas_reduction
 1m05.35s | 2190452 ko | ExtractionOCaml/bedrock2_solinas_reduction.ml
 1m03.87s | 2137192 ko | ExtractionOCaml/bedrock2_word_by_word_montgomery.ml
 1m01.18s | 2137308 ko | ExtractionOCaml/with_bedrock2_word_by_word_montgomery.ml
 0m58.53s | 2057100 ko | ExtractionOCaml/solinas_reduction.ml
 0m56.27s | 2063328 ko | ExtractionOCaml/with_bedrock2_unsaturated_solinas.ml
 0m55.76s | 1836424 ko | ExtractionOCaml/perf_word_by_word_montgomery.ml
 0m55.38s | 2030208 ko | ExtractionOCaml/word_by_word_montgomery.ml
 0m52.90s | 1413320 ko | ExtractionOCaml/perf_unsaturated_solinas
 0m51.44s | 2063536 ko | ExtractionOCaml/bedrock2_unsaturated_solinas.ml
 0m51.16s | 1950720 ko | ExtractionOCaml/bedrock2_base_conversion.ml
 0m50.96s | 1989736 ko | ExtractionOCaml/bedrock2_dettman_multiplication.ml
 0m49.61s | 1936244 ko | ExtractionOCaml/with_bedrock2_solinas_reduction.ml
 0m49.39s | 1936412 ko | ExtractionOCaml/with_bedrock2_saturated_solinas.ml
 0m49.38s | 1753040 ko | ExtractionOCaml/perf_unsaturated_solinas.ml
 0m48.72s | 1938204 ko | ExtractionOCaml/with_bedrock2_dettman_multiplication.ml
 0m48.29s | 1952524 ko | ExtractionOCaml/with_bedrock2_base_conversion.ml
 0m48.16s | 1938444 ko | ExtractionOCaml/bedrock2_saturated_solinas.ml
 0m47.28s | 1962520 ko | ExtractionOCaml/unsaturated_solinas.ml
 0m46.15s | 1823484 ko | ExtractionOCaml/base_conversion.ml
 0m42.74s | 1413036 ko | ExtractionOCaml/perf_word_by_word_montgomery
 0m41.95s | 1882704 ko | ExtractionOCaml/dettman_multiplication.ml
 0m38.36s | 1846056 ko | ExtractionOCaml/saturated_solinas.ml
 0m04.57s | 1035968 ko | Rewriter/PerfTesting/StandaloneOCamlMain.vo
 0m00.93s |  106556 ko | ExtractionOCaml/bedrock2_unsaturated_solinas.cmi
 0m00.90s |  102844 ko | ExtractionOCaml/bedrock2_fiat_crypto.cmi
 0m00.89s |  103608 ko | ExtractionOCaml/dettman_multiplication.cmi
 0m00.87s |  105352 ko | ExtractionOCaml/unsaturated_solinas.cmi
 0m00.84s |  102728 ko | ExtractionOCaml/fiat_crypto.cmi
 0m00.83s |  103608 ko | ExtractionOCaml/saturated_solinas.cmi
 0m00.83s |  103844 ko | ExtractionOCaml/with_bedrock2_fiat_crypto.cmi
 0m00.81s |  102720 ko | ExtractionOCaml/with_bedrock2_saturated_solinas.cmi
 0m00.80s |  103684 ko | ExtractionOCaml/bedrock2_saturated_solinas.cmi
 0m00.76s |  102640 ko | ExtractionOCaml/with_bedrock2_solinas_reduction.cmi
 0m00.76s |  107620 ko | ExtractionOCaml/with_bedrock2_unsaturated_solinas.cmi
 0m00.75s |  102300 ko | ExtractionOCaml/bedrock2_dettman_multiplication.cmi
 0m00.75s |  103592 ko | ExtractionOCaml/with_bedrock2_base_conversion.cmi
 0m00.75s |  102900 ko | ExtractionOCaml/with_bedrock2_word_by_word_montgomery.cmi
 0m00.74s |  102780 ko | ExtractionOCaml/bedrock2_base_conversion.cmi
 0m00.72s |  103088 ko | ExtractionOCaml/bedrock2_word_by_word_montgomery.cmi
 0m00.71s |  105644 ko | ExtractionOCaml/word_by_word_montgomery.cmi
 0m00.70s |  103272 ko | ExtractionOCaml/base_conversion.cmi
 0m00.69s |  103100 ko | ExtractionOCaml/with_bedrock2_dettman_multiplication.cmi
 0m00.67s |  102580 ko | ExtractionOCaml/bedrock2_solinas_reduction.cmi
 0m00.67s |  103236 ko | ExtractionOCaml/solinas_reduction.cmi
 0m00.42s |   58808 ko | ExtractionOCaml/perf_word_by_word_montgomery.cmi
 0m00.39s |   60084 ko | ExtractionOCaml/perf_unsaturated_solinas.cmi

```
</p>
</details>

src/CLI.v
@@ -17,6 +17,7 @@ Require Import Crypto.Util.Strings.NamingConventions.
 Require Import Crypto.Util.Option.
 Require Import Crypto.Util.OptionList.
 Require Import Crypto.Util.Strings.Show.
+Require Import Crypto.Util.Strings.Show.Enum.
 Require Import Crypto.Util.Strings.Sorting.
 Require Import Crypto.Util.Strings.ParseFlagOptions.
 Require Import Crypto.Util.DebugMonad.
@@ -44,6 +45,32 @@ Import
   Stringification.C.Compilers.
 
 Module ForExtraction.
+  Variant SynthesisKind : Set :=
+    | word_by_word_montgomery
+    | unsaturated_solinas
+    | saturated_solinas
+    | dettman_multiplication
+    | solinas_reduction
+    | base_conversion
+  .
+
+  Derive SynthesisKind_Listable SuchThat (@FinitelyListable SynthesisKind SynthesisKind_Listable) As SynthesisKind_FinitelyListable.
+  Proof. prove_ListableDerive. Qed.
+  Global Existing Instances SynthesisKind_Listable SynthesisKind_FinitelyListable.
+
+  Global Instance show_SynthesisKind : Show SynthesisKind.
+  Proof. prove_Show_enum (). Defined.
+  Global Instance show_lvl_SynthesisKind : ShowLevel SynthesisKind := show_SynthesisKind.
+
+  Definition parse_SynthesisKind_list : list (string * SynthesisKind)
+    := Eval vm_compute in
+      List.map
+        (fun r => (String.replace "_" "-" (show r), r))
+        (list_all SynthesisKind).
+
+  Definition parse_SynthesisKind_act : ParserAction SynthesisKind
+    := parse_strs parse_SynthesisKind_list.
+
   Definition parse_string_and {T} (parse_T : string -> option T) (s : string) : option (string * T)
     := option_map (@pair _ _ s) (parse_T s).
   Definition parse_Z (s : string) : option Z := parseZ_arith_strict s.
@@ -62,6 +89,9 @@ Module ForExtraction.
           ls <-- List.map ParseArithmetic.Q_to_Z_strict ls;
           Some ls).
 
+  Definition parse_SynthesisKind (s : string) : option SynthesisKind
+    := finalize parse_SynthesisKind_act s.
+
   Definition parse_list_REG (s : string) : option (list REG)
     := finalize (parse_comma_list parse_REG) s.
 
@@ -76,9 +106,6 @@ Module ForExtraction.
 
   Definition parse_callee_saved_registers (s : string) : option assembly_callee_saved_registers_opt
     := finalize parse_assembly_callee_saved_registers_opt s.
-
-  (* Workaround for lack of notation in 8.8 *)
-  Local Notation "x =? y" := (if string_dec x y then true else false) : string_scope.
 
   Definition parse_n (n : string) : option MaybeLimbCount
     := match parse_nat n with
@@ -301,6 +328,10 @@ Module ForExtraction.
                     end)%string
                 special_options)).
 
+  Definition synthesis_kind_spec : anon_argT
+    := ("synthesis_kind",
+         Arg.CustomSymbol parse_SynthesisKind_list,
+         ["The algorithm for field arithmetic.  Further options depend on the choice of algorithm, and can be viewed by passing -h after this argument.  Note that no options other than -h are permitted before this argument."]).
   Definition curve_description_spec : anon_argT
     := ("curve_description",
         Arg.String,
@@ -1003,6 +1034,7 @@ Module ForExtraction.
            end.
 
       Definition PipelineMain
+                 {prog_name_count : Arg.prog_name_countT}
                  {supported_languages : supported_languagesT}
                  {A}
                  {io_driver : IODriverAPI A}
@@ -1105,6 +1137,7 @@ Module ForExtraction.
         }.
 
     Definition PipelineMain
+               {prog_name_count : Arg.prog_name_countT}
                {supported_languages : supported_languagesT}
                {A}
                {io_driver : IODriverAPI A}
@@ -1147,6 +1180,7 @@ Module ForExtraction.
         }.
 
     Definition PipelineMain
+               {prog_name_count : Arg.prog_name_countT}
                {supported_languages : supported_languagesT}
                {A}
                {io_driver : IODriverAPI A}
@@ -1182,6 +1216,7 @@ Module ForExtraction.
         }.
 
     Definition PipelineMain
+               {prog_name_count : Arg.prog_name_countT}
                {supported_languages : supported_languagesT}
                {A}
                {io_driver : IODriverAPI A}
@@ -1228,6 +1263,7 @@ Module ForExtraction.
         }.
 
     Definition PipelineMain
+               {prog_name_count : Arg.prog_name_countT}
                {supported_languages : supported_languagesT}
                {A}
                {io_driver : IODriverAPI A}
@@ -1263,6 +1299,7 @@ Module ForExtraction.
       }.
 
     Definition PipelineMain
+               {prog_name_count : Arg.prog_name_countT}
                {supported_languages : supported_languagesT}
                {A}
                {io_driver : IODriverAPI A}
@@ -1331,6 +1368,7 @@ Module ForExtraction.
         }.
 
     Definition PipelineMain
+               {prog_name_count : Arg.prog_name_countT}
                {supported_languages : supported_languagesT}
                {A}
                {io_driver : IODriverAPI A}
@@ -1338,4 +1376,46 @@ Module ForExtraction.
       : A
       := Parameterized.PipelineMain argv.
   End BaseConversion.
+
+  (** The combined binary that delegates *)
+  Module FiatCrypto.
+    Definition PipelineMain
+      {supported_languages : supported_languagesT}
+      {A}
+      {io_driver : IODriverAPI A}
+      (argv : list string)
+      : A
+      := let spec
+           := {| Arg.named_args := []
+              ; Arg.anon_args := [synthesis_kind_spec]
+              ; Arg.anon_opt_args := []
+              ; Arg.anon_opt_repeated_arg := None |} in
+         match Arg.parse_argv (List.firstn 2 argv) spec with
+         | ErrorT.Success (tt as _named_data, anon_data, tt as _anon_opt_data, tt as _anon_opt_repeated_data)
+           => let synthesis_kind := anon_data in
+              let prog_name_count : Arg.prog_name_countT := 2%nat in
+              match synthesis_kind with
+              | word_by_word_montgomery
+                => WordByWordMontgomery.PipelineMain (prog_name_count:=prog_name_count) argv
+              | unsaturated_solinas
+                => UnsaturatedSolinas.PipelineMain (prog_name_count:=prog_name_count) argv
+              | saturated_solinas
+                => SaturatedSolinas.PipelineMain (prog_name_count:=prog_name_count) argv
+              | dettman_multiplication
+                => DettmanMultiplication.PipelineMain (prog_name_count:=prog_name_count) argv
+              | solinas_reduction
+                => SolinasReduction.PipelineMain (prog_name_count:=prog_name_count) argv
+              | base_conversion
+                => BaseConversion.PipelineMain (prog_name_count:=prog_name_count) argv
+              end
+         | ErrorT.Error err
+           => let display := Arg.show_list_parse_error spec err in
+              if Arg.is_real_error err
+              then error display
+              else (* just a requested help/usage message *)
+                write_stdout_then
+                  (List.map (fun s => s ++ String.NewLine)%string display)
+                  ret
+         end.
+  End FiatCrypto.
 End ForExtraction.
